proof/DenotationSpecsSimp.v
@@ -1,0 +1,161 @@
+Set Warnings "-notation-overridden,-parsing".
+From PLF Require Import Maps.
+From PLF Require Import CoreLangSimp.
+From PLF Require Import NormalTypeSystemSimp.
+From PLF Require Import LinearContext.
+From PLF Require Import RfTypeDef.
+From PLF Require Import TypeClosedSimp.
+From PLF Require Import TermOrdering.
+From PLF Require Import DenotationSimp.
+From PLF Require Import WellFormedSimp.
+From Coq Require Import Logic.FunctionalExtensionality.
+From Coq Require Import Logic.ClassicalFacts.
+From Coq Require Import Lists.List.
+From Coq Require Import FunInd.
+From Coq Require Import Recdef.
+
+Import CoreLangSimp.
+Import NormalTypeSystemSimp.
+Import LinearContext.
+Import RfTypeDef.
+Import TypeClosedSimp.
+Import DenotationSimp.
+Import WellFormedSimp.
+Import ListNotations.
+
+Global Hint Constructors well_formed_type: core.
+
+Lemma tmR_in_ctx_id_eq_c: forall st Gamma (id: string) c,
+    tmR_in_ctx_aux st Gamma (mk_eq_constant c) id ->
+    (forall e tau, tmR_in_ctx_aux st Gamma tau e <-> tmR_in_ctx_aux st Gamma tau (subst id c e)).
+Admitted.
+
+Lemma tmR_in_ctx_state_implies_subst: forall (st: state) a (c_a: constant) Gamma tau,
+    st a = c_a ->
+    l_find_right_most Gamma a = None ->
+    (forall e, tmR_in_ctx_aux st Gamma tau e <-> tmR_in_ctx_aux st Gamma tau ([a := c_a] e)).
+Admitted.
+
+
+(* Assume there is no dup in the context to simplify the proof. *)
+Lemma tmR_in_ctx_preserve_oarr: forall Gamma st x (tau_x: overbasety) e (tau: underty),
+    type_ctx_no_dup (Gamma <l> x :l: Oty tau_x) ->
+    tmR_in_ctx_aux st (Gamma <l> x :l: Oty tau_x) tau e ->
+    tmR_in_ctx_aux st Gamma (x o: tau_x o--> tau) (vlam x (o\_ tau_x _/) e).
+Proof with eauto.
+  intro Gamma.
+  induction Gamma; simpl; intros st x tau_x e tau Hctx HD.
+  - setoid_rewrite app_nil_l in HD. inversion HD; subst. constructor... constructor... constructor...
+    split.
+    + simpl. constructor... constructor... apply tmR_in_ctx_aux_implies_has_type in HD.
+      unfold lcontxt_to_basic_ctx in HD. unfold ncontxt_to_basic_ctx in HD. simpl in HD...
+    + intros c_x Hc_xD e3 Happ. inversion Happ; subst. simpl.
+      eapply step_preserve_under_denotation... eapply eta_reduction...
+      eapply step_preserve_under_denotation... eapply eta_application_const_to_lete_const...
+      assert (tmR_in_ctx_aux (x !-> c_x; st) [] tau (tlete x c_x e)) as HH... inversion HH; subst. inversion H0...
+  - destruct a as (a & tau_a).
+    inversion HD; subst.
+    + constructor...
+      (* apply denotation_ctx_implies_last_well_formed_type in HD... inversion HD; subst. *)
+      intros c_x Hc_xD.
+      eapply step_preserve_ctx_denotation. apply eta_lete_const_to_subst.
+      simpl... destruct (eqb_spec a x)... exfalso. eapply type_ctx_no_dup_fst_last_diff_name...
+      eapply step_preserve_ctx_denotation... apply eta_lete_const_to_subst_in_lam...
+      eapply IHGamma...
+      apply type_ctx_no_dup_ctx_sub with (Gamma1 := (a, Oty ({{v:T | phi}}))::nil)...
+    + constructor...
+      destruct H7 as (e_x_hat & He_x_hatD & HH).
+      exists e_x_hat. split...
+      intros e_x He_xD c_x Hc_xT Hc_xE.
+      eapply step_preserve_ctx_denotation... eapply eta_closed_term_can_captured_by_lam...
+      apply IHGamma...
+      apply type_ctx_no_dup_ctx_sub with (Gamma1 := (a, Uty ([[v:T | phi]]))::nil)...
+    + constructor...
+      intros e_x He_xD.
+      eapply step_preserve_ctx_denotation... eapply eta_closed_term_can_captured_by_lam...
+      apply IHGamma...
+      apply type_ctx_no_dup_ctx_sub with (Gamma1 := (a, Uty tau_x0)::nil)...
+Qed.
+
+Lemma tmR_in_ctx_preserve_arrarr: forall Gamma st x (tau_x: underty) e (tau: underty),
+    type_ctx_no_dup (Gamma <l> x :l: Uty tau_x) ->
+    tmR_in_ctx_aux st (Gamma <l> x :l: Uty tau_x) tau e ->
+    tmR_in_ctx_aux st Gamma (tau_x u--> tau) (vlam x (u\_ tau_x _/) e).
+Proof with eauto.
+  intro Gamma.
+  induction Gamma; simpl; intros st x tau_x e tau Hctx HD.
+  - setoid_rewrite app_nil_l in HD. setoid_rewrite app_nil_l in Hctx.
+Admitted.
+
+Lemma tmR_in_ctx_preserve_arrarr_application: forall Gamma st x (v1 v2: value) tau tau1,
+    (* ctx_inv Gamma -> *)
+    tmR_in_ctx_aux st Gamma (tau1 u--> tau) v1 ->
+    tmR_in_ctx_aux st Gamma tau1 v2 ->
+    tmR_in_ctx_aux st Gamma tau (tletapp x v1 v2 x).
+Proof with eauto.
+  intro Gamma.
+  induction Gamma; simpl; intros st x v1 v2 tau tau_x Hv1D Hv2D.
+  - inversion Hv1D; subst. inversion Hv2D; subst. clear Hv1D Hv2D. constructor... inversion H; subst. inversion H3; subst. clear H H3. inversion H0; subst. clear H0.
+    destruct H2 as (Hv1T & HH). destruct (value_value_is_application x v1 v2) as (e3 & (He3app & He3E)).
+    eapply HH with (e3:=e3) in H4... constructor... eapply step_preserve_under_denotation... destruct He3E...
+  - destruct a as (a & tau_a).
+    inversion Hv1D; subst.
+    + constructor... { inversion H3; subst... } inversion Hv2D; subst.
+      intros c_x He_xD.
+      (* make HHv1 and HHv2 to value. *)
+      assert (tmR_in_ctx_aux (a !-> c_x; st) Gamma (tau_x u--> tau) ([a := c_x] v1)) as HHv1...
+      { eapply step_preserve_ctx_denotation... apply eta_lete_const_to_subst. } clear H7.
+      assert (tmR_in_ctx_aux (a !-> c_x; st) Gamma tau_x ([a := c_x] v2)) as HHv2...
+      { eapply step_preserve_ctx_denotation... apply eta_lete_const_to_subst. } clear H11.
+      eapply step_preserve_ctx_denotation. apply eta_lete_const_to_subst. rewrite subst_letapp_penetrate.
+      eapply IHGamma...
+    + constructor... { inversion H3; subst... }
+      destruct H7 as (e_x_hat & He_x_hatD & HH).
+      exists e_x_hat. split...
+      intros e_x He_xD c_x Hc_xT Hc_xE.
+      (* (need context inv) *)
+Admitted.
+
+Lemma tmR_in_ctx_preserve_oarr_c_application: forall Gamma st x (v1: value) (c2: constant) tau a T phi,
+    tmR_in_ctx_aux st Gamma (a o: {{v: T | phi}} o--> tau) v1 ->
+    tmR_in_ctx_aux st Gamma ([[v: T | phi]]) c2 ->
+    tmR_in_ctx_aux st Gamma (under_subst_c a c2 tau) (tletapp x v1 c2 x).
+Admitted.
+
+Lemma tmR_in_ctx_preserve_oarr_var_application: forall Gamma st x (v1: value) (name2: string) tau a T phi,
+    tmR_in_ctx_aux st Gamma (a o: {{v: T | phi}} o--> tau) v1 ->
+    tmR_in_ctx_aux st Gamma ([[v: T | phi]]) name2 ->
+    tmR_in_ctx_aux st Gamma (under_subst_id a name2 tau) (tletapp x v1 name2 x).
+Admitted.
+
+Lemma tmR_in_ctx_preserve_matchb_true: forall Gamma st (v: value) e1 e2 tau,
+    tmR_in_ctx_aux st Gamma (mk_eq_constant true) v ->
+    tmR_in_ctx_aux st Gamma tau e1 ->
+    tmR_in_ctx_aux st Gamma tau (tmatchb v e1 e2).
+Proof with eauto.
+  intros Gamma st v e1 e2 tau Hv He1.
+  assert ((exists n : bool, v = n) \/ (exists name : string, v = name)) as HH. apply tmR_in_ctx_aux_implies_has_type in Hv. inversion Hv; subst. apply bool_value_cid_exists in H1...
+  destruct HH.
+  - destruct H as (b & Hb); subst. apply mk_eq_constant_is_itsefl_in_ctx in Hv. rewrite Hv.
+    eapply step_preserve_ctx_denotation... apply eta_matchb_true...
+  - destruct H as (id & Hid); subst. rewrite tmR_in_ctx_id_eq_c... simpl. rewrite eqb_refl.
+    apply step_preserve_ctx_denotation with (e:= ([id := true] e1))... apply eta_matchb_true...
+    rewrite <- tmR_in_ctx_id_eq_c...
+Qed.
+
+
+Lemma tmR_in_ctx_preserve_matchb_false: forall st Gamma (v: value) e1 e2 tau,
+    tmR_in_ctx_aux st Gamma (mk_eq_constant false) v ->
+    tmR_in_ctx_aux st Gamma tau e2 ->
+    tmR_in_ctx_aux st Gamma tau (tmatchb v e1 e2).
+Proof with eauto.
+  intros st Gamma v e1 e2 tau Hv He1.
+  assert ((exists n : bool, v = n) \/ (exists name : string, v = name)) as HH. apply tmR_in_ctx_aux_implies_has_type in Hv. inversion Hv; subst. apply bool_value_cid_exists in H1...
+  destruct HH.
+  - destruct H as (b & Hb); subst. apply mk_eq_constant_is_itsefl_in_ctx in Hv. rewrite Hv.
+    eapply step_preserve_ctx_denotation... apply eta_matchb_false...
+  - destruct H as (id & Hid); subst. rewrite tmR_in_ctx_id_eq_c... simpl. rewrite eqb_refl.
+    apply step_preserve_ctx_denotation with (e:= ([id := false] e2))... apply eta_matchb_false...
+    rewrite <- tmR_in_ctx_id_eq_c...
+Qed.
+
