proof/Soundness.v
@@ -6,6 +6,7 @@ From PLF Require Import LinearContext.
 From PLF Require Import RfTypeDef.
 From PLF Require Import TypeClosedSimp.
 From PLF Require Import DenotationSimp.
+From PLF Require Import DenotationSpecsSimp.
 From PLF Require Import SubtypingSimp.
 From PLF Require Import TypingRules.
 From Coq Require Import Logic.FunctionalExtensionality.
@@ -19,6 +20,7 @@ Import DenotationSimp.
 Import WellFormedSimp.
 Import TypeDisj.
 Import SubtypingSimp.
+Import DenotationSpecsSimp.
 Import TypingRules.
 Import ListNotations.
 
@@ -45,64 +47,66 @@ Global Hint Resolve ctx_inv_implies_type_closed_last: core.
 Global Hint Rewrite app_nil_r: core.
 
 Theorem soundness: forall (Gamma: context) (e: tm) (uty:underty),
-    Gamma \C- e \Tin uty -> tmR_in_ctx Gamma uty e.
+    Gamma \C- e \Tin uty -> tmR_in_ctx_all_st Gamma uty e.
 Proof with eauto.
   apply (term_under_type_chek_rec
-           (fun Gamma v uty H => tmR_in_ctx Gamma uty (tvalue v))
-           (fun Gamma e uty H => tmR_in_ctx Gamma uty e)); intros Gamma.
+           (fun Gamma v uty H => tmR_in_ctx_all_st Gamma uty (tvalue v))
+           (fun Gamma e uty H => tmR_in_ctx_all_st Gamma uty e)); intros Gamma.
   (* constant *)
-  - intros c Hinv.
-    apply tmR_in_ctx_pre_weakening with (Gamma1 := Gamma) (Gamma2 := l_empty); auto. rewrite app_nil_r... constructor...
+  - intros c Hinv st.
+    apply tmR_in_ctx_pre_weakening with (Gamma1 := Gamma) (Gamma2 := l_empty); auto. rewrite app_nil_r...
   (* op *)
-  - intros op a b (Hinv & Hclosed) Hab. apply tmR_in_ctx_pre_weakening with (Gamma1 := Gamma) (Gamma2 := l_empty); auto.
-    rewrite app_nil_r... constructor...
+  - intros op a b (Hinv & Hclosed) Hab st. apply tmR_in_ctx_pre_weakening with (Gamma1 := Gamma) (Gamma2 := l_empty); auto.
+    rewrite app_nil_r...
   (* var over base *)
-  - intros T x Hinv (phi & Hfind). apply l_find_right_most_some_spec in Hfind.
+  - intros T x Hinv (phi & Hfind) st. apply l_find_right_most_some_spec in Hfind.
     destruct Hfind as (Gamma1 & Gamma2 & Hctxconcat & HGamma2). subst.
     rewrite app_assoc. rewrite app_assoc in Hinv. inversion Hinv; subst.
     eapply tmR_in_ctx_post_weakening with (Gamma1 := (Gamma1 ++ ((x, Oty ({{v:T | phi}}))::nil))) (Gamma2 := Gamma2)...
     apply over_variable_has_eq_type_in_ctx.
   (* var under base *)
-  - intros T x (Hinv & Hclosed) (phi & Hfind). apply l_find_right_most_some_spec in Hfind.
+  - intros T x (Hinv & Hclosed) (phi & Hfind) st. apply l_find_right_most_some_spec in Hfind.
     destruct Hfind as (Gamma1 & Gamma2 & Hctxconcat & HGamma2). subst.
     rewrite app_assoc. rewrite app_assoc in Hinv.
     eapply tmR_in_ctx_post_weakening with (Gamma1 := (Gamma1 ++ ((x, Uty ([[v:T | phi]]))::nil))) (Gamma2 := Gamma2)...
     apply under_variable_has_eq_type_in_ctx...
   (* var under arrarr *)
-  - intros x t1 t2 (Hinv & Hclosed) Hfind. apply l_find_right_most_some_spec in Hfind.
+  - intros x t1 t2 (Hinv & Hclosed) Hfind st. apply l_find_right_most_some_spec in Hfind.
     destruct Hfind as (Gamma1 & Gamma2 & Hctxconcat & HGamma2). subst.
     eapply tmR_in_ctx_post_weakening with (Gamma1:= Gamma1 ++ ((x, Uty (t1 u--> t2))::nil)) (Gamma2 := Gamma2)... rewrite app_assoc...
     + eapply ctx_inv_implies_mem_fresh_and_close...
     + apply under_variable_has_same_type_in_ctx...
   (* var under oarr *)
-  - intros x a tau_a tau_b (Hinv & Hclosed) Hfind. apply l_find_right_most_some_spec in Hfind.
+  - intros x a tau_a tau_b (Hinv & Hclosed) Hfind st. apply l_find_right_most_some_spec in Hfind.
     destruct Hfind as (Gamma1 & Gamma2 & Hctxconcat & HGamma2). subst.
     eapply tmR_in_ctx_post_weakening with (Gamma1:= Gamma1 ++ ((x, Uty (a o: tau_a o--> tau_b))::nil)) (Gamma2 := Gamma2)... rewrite app_assoc...
     + eapply ctx_inv_implies_mem_fresh_and_close...
     + apply under_variable_has_same_type_in_ctx...
   (* lam *)
-  - intros x tau_x e tau (Hinv & Hclosed) He HeD.
+  - intros x tau_x e tau (Hinv & Hclosed) He HeD st.
     assert (well_formed (Gamma <l> x :l: tau_x) tau) as HH. apply type_judgement_implies_inv in He...
     destruct HH as (Hinv' & Hclosed'). apply tmR_in_ctx_preserve_oarr... inversion Hinv'; subst...
-  - intros x tau_x e tau Hwf He HeD.
+  - intros x tau_x e tau Hwf He HeD st.
     assert (well_formed (Gamma <l> x :l: tau_x) tau) as HH. apply type_judgement_implies_inv in He...
     destruct HH as (Hinv' & Hclosed').
     apply tmR_in_ctx_preserve_arrarr... inversion Hinv'; subst...
   (* value *)
   - auto.
   (* err *)
-  - intros T (Hinv & Hclosed).
-    assert (tmR_in_ctx l_empty (mk_bot T) texn)... unfold mk_bot.
+  - intros T (Hinv & Hclosed) st.
+    assert (tmR_in_ctx_aux st l_empty (mk_bot T) texn)... unfold mk_bot.
     repeat constructor... intros. inversion H0.
     apply tmR_in_ctx_pre_weakening with (Gamma1 := Gamma) (Gamma2 := l_empty)... rewrite app_nil_r...
     constructor...
   (* sub *)
-  - intros e tau1 tau2 (Hinv & Hclosed) He HeD Hsub.
+  - intros e tau1 tau2 (Hinv & Hclosed) He HeD Hsub st.
     apply is_subtype_spec with (e:=e) in Hsub...
     eapply tmR_in_ctx_pre_weakening with (Gamma1 := Gamma) (Gamma2 := l_empty)... apply app_nil_r...
-    inversion Hsub; subst. eapply denotation_is_closed...
+    assert (tmR_in_ctx_aux empstate l_empty tau2 e)... inversion H; subst. eapply denotation_is_closed...
+    (* unfold tmR_in_ctx_all_st in Hsub. eapply denotation_is_closed... remember (Hsub st). *)
+    (* inversion (Hsub st). subst. eapply denotation_is_closed... *)
   (* eq *)
-  - intros e tau1 tau2 (Hinv & Hclosed) He HeD Hsub1 Hsub2.
+  - intros e tau1 tau2 (Hinv & Hclosed) He HeD Hsub1 Hsub2 st.
     eapply is_subtype_spec...
   (* merge *)
   - intros e tau1 tau2 tau3 (Hinv & Hclosed) He1 He1D He2 He2D Hdisj. unfold disjunct in Hdisj. rewrite <- Hdisj...
@@ -126,8 +130,8 @@ Proof with eauto.
     assert (ctx_inv Gamma). eapply type_judgement_implies_inv... constructor...
     eapply tletapp_oarr_ctx_inv_implies_safe_dropping_1_to_1...
   (* matchb true *)
-  - intros v e1 e2 tau (Hinv & Hclosed) Hv HvD He1 He1D. eapply tmR_in_ctx_preserve_matchb_true...
-  - intros v e1 e2 tau (Hinv & Hclosed) Hv HvD He1 He1D. eapply tmR_in_ctx_preserve_matchb_false...
+  - intros v e1 e2 tau (Hinv & Hclosed) Hv HvD He1 He1D st. eapply tmR_in_ctx_preserve_matchb_true...
+  - intros v e1 e2 tau (Hinv & Hclosed) Hv HvD He1 He1D st. eapply tmR_in_ctx_preserve_matchb_false...
 Qed.
 
 Lemma coverage: forall (e: tm) (T:base_ty) (phi: constant -> Prop),
@@ -135,8 +139,8 @@ Lemma coverage: forall (e: tm) (T:base_ty) (phi: constant -> Prop),
     forall (c: constant), empty |- (vconst c) \Vin T -> phi c -> e -->* vconst c .
 Proof with eauto.
   intros.
-  apply soundness in H.
-  inversion H; subst.
+  apply soundness in H. remember (H empstate) as HH.
+  inversion HH; subst.
   inversion H2; subst. simpl in H2, H5.
   destruct H5 as (_ & _ & Hprop).
   apply Hprop; auto.
