proof/TypeDisj.v
@@ -19,6 +19,6 @@ Import ListNotations.
 (* disjunction judgement *)
 
 Definition disjunct (Gamma: context) (tau1 tau2 tau3: underty) :=
-  (forall e, tmR_in_ctx Gamma tau1 e /\ tmR_in_ctx Gamma tau2 e <-> tmR_in_ctx Gamma tau3 e).
+  (forall e, tmR_in_ctx_all_st Gamma tau1 e /\ tmR_in_ctx_all_st Gamma tau2 e <-> tmR_in_ctx_all_st Gamma tau3 e).
 
 Notation "Gamma '\C-' tau1 '\tyor' tau2 '\tyeq' tau3 " := (disjunct Gamma tau1 tau2 tau3) (at level 40).
